casestudy/imp/Common.v
@@ -1,0 +1,3 @@
+(* Things that are shared by all families *)
+
+Definition ident := positive.
