casestudy/imp/base/Impminor.v
@@ -1,0 +1,67 @@
+Inductive constant : Type :=
+  | Ointconst: int -> constant     (**r integer constant *)
+  | Oaddrsymbol: ident -> ptrofs -> constant (**r address of the symbol plus the offset *)
+  | Oaddrstack: ptrofs -> constant.   (**r stack pointer plus the given offset *)
+
+Inductive unary_operation : Type :=
+  | Ocast8unsigned: unary_operation        (**r 8-bit zero extension  *)
+  | Ocast8signed: unary_operation          (**r 8-bit sign extension  *)
+  | Ocast16unsigned: unary_operation       (**r 16-bit zero extension  *)
+  | Ocast16signed: unary_operation         (**r 16-bit sign extension *)
+  | Onegint: unary_operation               (**r integer opposite *)
+  | Onotint: unary_operation               (**r bitwise complement  *)
+  | Onegl: unary_operation                 (**r long integer opposite *)
+  | Onotl: unary_operation                 (**r long bitwise complement *)
+  | Ointoflong: unary_operation            (**r long to int *)
+  | Olongofint: unary_operation            (**r signed int to long *)
+  | Olongofintu: unary_operation           (**r unsigned int to long *)
+
+Inductive binary_operation : Type :=
+  | Oadd: binary_operation                 (**r integer addition *)
+  | Osub: binary_operation                 (**r integer subtraction *)
+  | Omul: binary_operation                 (**r integer multiplication *)
+  | Odiv: binary_operation                 (**r integer signed division *)
+  | Odivu: binary_operation                (**r integer unsigned division *)
+  | Omod: binary_operation                 (**r integer signed modulus *)
+  | Omodu: binary_operation                (**r integer unsigned modulus *)
+  | Oand: binary_operation                 (**r integer bitwise ``and'' *)
+  | Oor: binary_operation                  (**r integer bitwise ``or'' *)
+  | Oxor: binary_operation                 (**r integer bitwise ``xor'' *)
+  | Oshl: binary_operation                 (**r integer left shift *)
+  | Oshr: binary_operation                 (**r integer right signed shift *)
+  | Oshru: binary_operation                (**r integer right unsigned shift *)
+  | Oaddl: binary_operation                (**r long addition *)
+  | Osubl: binary_operation                (**r long subtraction *)
+  | Omull: binary_operation                (**r long multiplication *)
+  | Odivl: binary_operation                (**r long signed division *)
+  | Odivlu: binary_operation               (**r long unsigned division *)
+  | Omodl: binary_operation                (**r long signed modulus *)
+  | Omodlu: binary_operation               (**r long unsigned modulus *)
+  | Oandl: binary_operation                (**r long bitwise ``and'' *)
+  | Oorl: binary_operation                 (**r long bitwise ``or'' *)
+  | Oxorl: binary_operation                (**r long bitwise ``xor'' *)
+  | Oshll: binary_operation                (**r long left shift *)
+  | Oshrl: binary_operation                (**r long right signed shift *)
+  | Oshrlu: binary_operation               (**r long right unsigned shift *)
+  | Ocmp: comparison -> binary_operation   (**r integer signed comparison *)
+  | Ocmpu: comparison -> binary_operation  (**r integer unsigned comparison *)
+  | Ocmpl: comparison -> binary_operation  (**r long signed comparison *)
+  | Ocmplu: comparison -> binary_operation. (**r long unsigned comparison *)
+
+Inductive expr : Type :=
+  | Evar : ident -> expr
+  | Econst : constant -> expr
+  | Eunop : unary_operation -> expr -> expr
+  | Ebinop : binary_operation -> expr -> expr -> expr
+  | Eload : memory_chunk -> expr -> expr.
+                           
+Inductive stmt : Type :=
+  | Sskip: stmt
+  | Sassign : ident -> expr -> stmt
+  | Sseq: stmt -> stmt -> stmt
+  | Sifthenelse: expr -> stmt -> stmt -> stmt
+  | Sloop: stmt -> stmt
+  | Sblock: stmt -> stmt
+  | Sexit: nat -> stmt
+  | Sswitch: bool -> expr -> list (Z * nat) -> nat -> stmt
+  | Sreturn: option expr -> stmt
