casestudy/imp/base/Linear.v
@@ -1,0 +1,15 @@
+Definition label := positive.
+
+Inductive instruction: Type :=
+  | Lgetstack: slot -> Z -> typ -> mreg -> instruction
+  | Lsetstack: mreg -> slot -> Z -> typ -> instruction
+  | Lop: operation -> list mreg -> mreg -> instruction
+  | Lload: memory_chunk -> addressing -> list mreg -> mreg -> instruction
+  | Lstore: memory_chunk -> addressing -> list mreg -> mreg -> instruction
+  | Llabel: label -> instruction
+  | Lgoto: label -> instruction
+  | Lcond: condition -> list mreg -> label -> instruction
+  | Ljumptable: mreg -> list label -> instruction
+  | Lreturn: instruction.
+
+Definition code: Type := list instruction.
