casestudy/imp/base/Mach.v
@@ -1,0 +1,18 @@
+Definition label := positive.
+
+Inductive instruction: Type :=
+  | Mgetstack: ptrofs -> typ -> mreg -> instruction
+  | Msetstack: mreg -> ptrofs -> typ -> instruction
+  | Mgetparam: ptrofs -> typ -> mreg -> instruction
+  | Mop: operation -> list mreg -> mreg -> instruction
+  | Mload: memory_chunk -> addressing -> list mreg -> mreg -> instruction
+  | Mstore: memory_chunk -> addressing -> list mreg -> mreg -> instruction
+  | Mlabel: label -> instruction
+  | Mgoto: label -> instruction
+  | Mcond: condition -> list mreg -> label -> instruction
+  | Mjumptable: mreg -> list label -> instruction
+  | Mreturn: instruction.
+
+Definition code := list instruction.
+
+
