NOTES.md
@@ -1,0 +1,20 @@
+
+
+1. Create the data pipeline for the compiler architecture
+   The pipeline is similar to the pipeline in CompCert.
+   We compile to Cminor (ImpMinor) -> CSel (ImpSel) -> RTL (ImpRTL) -> LTL (ImpLTL)
+   We can create all the inductive types and figure out how reuse with nested family
+   polymorphism will work.
+2. We want to have a syntax-directed algorithm (like [| e |]) for compiling nested
+   family polymorphism to vanilla Coq terms/modules. The problem is that we might
+   need to prove that this algorithm is correct... or we can say "This is just a
+   demonstration of the algorithm" - I'd personally prefer if we could prove this.
+   In some sense, proving this algorithm would be the equivalent of writing the
+   implementation in MetaCoq and proving the actual compilation algorithm correct.
+3. I think the processor-dependent style of types can be a good room to show case
+   family polymorphism. Because in some sense that is a kind of reuse/abstraction? 
+
+Q: 
+1. In some cases, it doens't make sense to have an IR when the features are small.
+   Can a family add a new IR?
+2. Do we need a backend compiler for the casestudy? e.g Arm?
