casestudy/imp/Denotational.v
@@ -1,1 +1,0 @@
-(* Imp w/ denotational demantics *)
